Replaced SIZE with size throughout Prim

prim/prim_constants.v
@@ -1,20 +1,20 @@
 Require Export VST.floyd.proofauto.
 
-Definition SIZE := 8 : Z.
+Definition size := 8 : Z.
 Definition inf := 2147483646 : Z.
 (* Int.max_signed - 1 *)
 
-Lemma SIZE_eq: SIZE = 8.
+Lemma size_eq: size = 8.
 Proof. auto. Qed.
 
 Lemma inf_eq: inf = 2147483646. 
 Proof. auto. Qed.
 
-Lemma SIZE_rep': 0 < SIZE <= Int.max_signed.
+Lemma size_rep': 0 < size <= Int.max_signed.
 Proof. compute; split; [trivial | inversion 1]. Qed.
 
-Lemma SIZE_rep: 0 <= SIZE <= Int.max_signed.
-Proof. pose proof SIZE_rep'. lia. Qed.
+Lemma size_rep: 0 <= size <= Int.max_signed.
+Proof. pose proof size_rep'. lia. Qed.
 
 Lemma inf_rep: 0 <= inf <= Int.max_signed.
 Proof. compute; split; inversion 1. Qed.
@@ -25,5 +25,5 @@ Proof.
   compute; split; inversion 1.
 Qed.
 
-Global Opaque SIZE.
+Global Opaque size.
 Global Opaque inf.
